{{< include /pages/_latex-macros.qmd >}}
---
title: "Danilevsky's Algorithm"
filters:
    - pseudocode
---

## Abstract

{Danilevsky} is a method to compute the coefficients of the {characteristic-polynomial} for a square matrix.

It isn't well known, so we review how it works for real-valued matrices.

We then go on to explain how it applies explicitly to bit-matrices, i.e., matrices over {gf2}, the simplest [Galois field] with just two elements 0 & 1 where addition/subtraction and multiplication/division operations are all done mod two which keeps everything closed in the set $\{0,1\}$.

## Characteristic Polynomials

Recall that $\lambda$ is an _eigenvalue_ of $A$, an $n \times n$ matrix, if there is an non-zero vector $v$ (an _eigenvector_) such that:
$$
  A \cdot v = \lambda v.
$$
Solving that equation is equivalent to finding solutions for the linear system
$$
  (A - \lambda I) v = 0.
$$
which has solutions if and only if $A - \lambda I$ is singular so
$$
   |A - \lambda I| = 0
$$
where we are using $|\cdot|$ to denote the determinant.

The characteristic polynomial of $A$ is defined by the determinant $|A - \lambda I|$ thought of as a function of $\lambda$:
$$
  c(\lambda) = |A - \lambda I|.
$$
Expanding the determinant, you can explicitly get a few of the terms in this polynomial as
$$
  c(\lambda) = (-\lambda)^n  + tr(A)(-\lambda)^{n-1} + \cdots + \det(A)
$$
where $tr(A)$ is the trace of the matrix $A$.
However, it is not practical to compute all the terms in the polynomial by brute force expansion like this.

Even if we have all the coefficients in the characteristic polynomial, getting the eigenvalues means solving
$$
  c(\lambda) = 0.
$$
However, extracting the roots of a high-order polynomial is very difficult.
For this reason, the method is only practical for the small matrices that turn up in homework exercises!

However, the {characteristic-polynomial} is a valuable structure for other purposes.
For one thing, the well-known {Cayley-Hamilton} theorem tells us that the characteristic polynomial is an {annihilating-polynomial} for the matrix.
Thus
$$
  c(A) = 0.
$$
This result is helpful in various applications.
For this reason, we are still interested in computing the coefficients $c_i$ of the characteristic polynomial written as
$$
  c(\lambda) = \lambda^n + c_{n-1} \lambda^{n-1} + \cdots + c_1 \lambda + c_0.
$$
(where without loss of generality, we take $c_n = 1$)

## Companion Matrices

Investigating square matrices of size $n$ led us to consider polynomials of order $n$.
How about the reverse?
If you have an arbitrary polynomial of the form
$$
  c(\lambda) = \lambda^n + c_{n-1} \lambda^{n-1} + \cdots + c_1 \lambda + c_0.
$$
Is there a matrix with that as its characteristic polynomial?

Here is one we will show works:
$$
C =
\begin{bmatrix}
-c_{n-1} & -c_{n-2} & -c_{n-3} & \ldots & & -c_2 & -c_1 & -c_0 \\
1        & 0        & 0        & \ldots & & 0    & 0    & 0    \\
0        & 1        & 0        & \ldots & & 0    & 0    & 0    \\
         &          &          & \ldots                        \\
0        & 0        & 0        & \ldots & & 1    & 0    & 0    \\
0        & 0        & 0        & \ldots & & 0    & 1    & 0
\end{bmatrix}
$$
This $C$ has ones on the sub-diagonal and the polynomial coefficients (with a minus sign) along the first row.
It is an upper {Hessenberg} matrix.

Computing the determinant is difficult for all but the smallest _general_ matrices.
However, getting the determinant for _triangular_ matrices is trivial, as you only need to multiply the elements on the diagonal.
{Hessenberg} matrices are _almost_ triangular and also quite amenable when it comes to computing determinants.

To see that our $C$ has the characteristic polynomial, we want to consider the determinant:
$$
|\lambda I - C| =
\begin{vmatrix}
\lambda+c_{n-1}     & c_{n-2}  & c_{n-3} & \ldots & & c_2 & c_1      & c_0    \\
1        & \lambda  & 0                  & \ldots & & 0    & 0       & 0      \\
0        & 1        & \lambda            & \ldots & & 0    & 0       & 0      \\
         &          &                    & \ldots                             \\
0        & 0        & 0                  & \ldots & & 1    & \lambda & 0      \\
0        & 0        & 0                  & \ldots & & 0    & 1       & \lambda
\end{vmatrix}
$$
When you expand that determinant by the first row, then you get
$$
(\lambda + c_{n-1})
\begin{vmatrix}
& \lambda  & 0                  & \ldots & & 0    & 0       & 0      \\
& 1        & \lambda            & \ldots & & 0    & 0       & 0      \\
&          &                    & \ldots                             \\
& 0        & 0                  & \ldots & & 1    & \lambda & 0      \\
& 0        & 0                  & \ldots & & 0    & 1       & \lambda
\end{vmatrix}
+ c_{n-2}
\begin{vmatrix}
& 1  & 0                        & \ldots & & 0    & 0       & 0      \\
& 0        & \lambda            & \ldots & & 0    & 0       & 0      \\
&          &                    & \ldots                             \\
& 0        & 0                  & \ldots & & 1    & \lambda & 0      \\
& 0        & 0                  & \ldots & & 0    & 1       & \lambda
\end{vmatrix}
+ \dots
+ c_0
\begin{vmatrix}
& 1        & 0                  & \ldots & & 0    & 0       & 0         \\
& 0        & 1                  & \ldots & & 0    & 0       & 0         \\
&          &                    & \ldots                                \\
& 0        & 0                  & \ldots & &      & 1       & \lambda   \\
& 0        & 0                  & \ldots & & 0    & 0       & 1
\end{vmatrix}
$$
The {co-factors} are all $(n-1) \times (n-1)$ triangular so have readily computed determinants which means that:
$$
|\lambda I - C| =  (\lambda + c_{n-1}) \lambda^{n-1} + c_{n-2} \lambda^{n-2} + \cdots + c_0.
$$
That is exactly the form we want.

NOTE: You can make the same determinant expansion argument if the polynomial coefficients were in the final column instead of the top row.
That is the version seen in some expositions.

$C$ is a "companion" for the polynomial $c(\lambda)$ and is known as a {companion-matrix.

### Frobenius Form

First, note that you can create many others once you have a matrix (like the $C$ above) with the desired characteristic polynomial.
The reason is that {similar-matrices} all have the same characteristic polynomial.
So if $M$ is any invertible $n \times n$ matrix, then $M^{-1} \cdot C \cdot M$ will have the same characteristic polynomial as $C$.

Now let $A$ be an arbitrary $n \times n$ matrix.

A natural question then is whether you can find some invertible $M$ such that $C = M^{-1} \cdot A \cdot M$ is in {companion-matrix} form. If so, you can read the characteristic polynomial coefficients for $A$ off the top row of $C$.

Generally, this isn't quite possible, but instead, you can always get to {Frobenius-form}.
A Frobenius form matrix is block-diagonal, where each block is a {companion-matrix.

So there is always some $M$ such that
$$
A = M^{-1} \cdot F \cdot M.
$$
And the matrix $F$ has the block-diagonal form
$$
F =
\begin{bmatrix}
C_0 & 0   & 0 & \ldots & 0 & 0 \\
0   & C_1 & 0 & \ldots & 0 & 0 \\
    &     &   & \ldots         \\
0   & 0   & 0 & \ldots & 0 & C_{k-1}
\end{bmatrix}
$$
and each of the $k$ diagonal blocks is a {companion-matrix.

You can read off the coefficients of each block to get a set of characteristic polynomials $c_i(\lambda)$ for $i = 0, \ldots, k-1$.
Then the characteristic polynomial of $F$ and hence by similarity, $A$ is just:
$$
c(\lambda) = \prod_{i = 0}^{k-1} c_i(\lambda).
$$

If $A$ is an arbitrary real-valued $n \times n$ matrix, {Danilevsky} applies a sequence of similarity transformations that, step by step, efficiently moves it to {Frobenius-form}.


## Danilevsky for Real Matrices

We will describe how the algorithm works for an $n \times n$ matrix $A$ with elements in $\R$.
The algorithm can be written as

$$
A = A_1 \rightarrow A_2 \rightarrow \ldots \rightarrow A_n
$$
where that final matrix, $A_n$, is in Frobenius form.
At each stage, $A_{k+1}$ is constructed from its predecessor $A_{k}$ via a similarity transformation:
$$
A_{k+1} = M^{-1}_{k} \cdot A_k \cdot M_k.
$$
Here "$\cdot$" denotes matrix multiplication.

The algorithm is efficient because we can readily construct the $M_k$'s and their inverses.
Moreover, they are  _sparse_ matrices, meaning those two matrix multiplications can be performed quickly in $O(n^2)$ operations instead of the usual $O(n^3)$.

Starting with a general matrix such as

$$
A := A_1 =
\begin{bmatrix}
a_{11} & a_{12} & a_{13} & \ldots & a_{1n-2} & a_{1n-1} & a_{1n} \\
a_{21} & a_{22} & a_{23} & \ldots & a_{2n-2} & a_{2n-1} & a_{2n} \\
& & & \ldots \\
& & & \ldots \\
a_{n-11} & a_{n-12} & a_{n-13} & \ldots & a_{n-1n-2} & a_{n-1n-1} & a_{n-1n} \\
a_{n1} & a_{n2} & a_{n3} & \ldots & a_{nn-2} & a_{nn-1} & a_{nn}
\end{bmatrix}
$$

we would love to get to the companion matrix form

$$
A_n =
\begin{bmatrix}
c_1 & c_2 & c_3 & \ldots & & c_{n-2} & c_{n-1} & c_{n} \\
1 & 0 & 0 & \ldots & & 0 & 0 & 0 \\
& & & \ldots \\
& & & \ldots \\
0 & 0 & 0 & \ldots & & 1 & 0 & 0 \\
0 & 0 & 0 & \ldots & & 0 & 1 & 0 \\
\end{bmatrix}
$$

The characteristic polynomial for $A$ is then

$$
c(\lambda) = 1 + c_1 \lambda + c_2 \lambda^2 + \cdots + c_{n-1} \lambda^{n-1} + c_{n} \lambda^{n}.
$$

To get things rolling, we need to construct a matrix $M$ such that $A \cdot M$ is one step closer to companion matrix form (we are dropping the subscripts on the matricesâ€”in a computer implementation the matrices mostly just get updated in-place anyway).

Our aim is to find $M$ so that $B := A \cdot M$ has the form

$$
\begin{bmatrix}
b_{11} & b_{12} & b_{13} & \ldots & b_{1n-2} & b_{1n-1} & b_{1n} \\
b_{21} & b_{22} & b_{23} & \ldots & b_{2n-2} & b_{2n-1} & b_{2n} \\
& & & \ldots \\
& & & \ldots \\
b_{n-11} & b_{n-12} & b_{n-13} & \ldots & b_{n-1n-2} & b_{n-1n-1} & b_{n-1n} \\
0 & 0 & 0 & \ldots & 0 & 1 & 0
\end{bmatrix}
$$

Assuming that $a_{nn-1} \neq 0$, an appropriate $M$ is

$$
M =
\begin{bmatrix}
1 & 0 & 0 & \ldots & 0 & 0 & 0 \\
0 & 1 & 0 & \ldots & 0 & 0 & 0 \\
& & & \ldots \\
& & & \ldots \\
\frac{-a_{n1}}{a_{nn-1}} & \frac{-a_{n2}}{a_{nn-1}} & \frac{-a_{n3}}{a_{nn-1}} & \ldots & \frac{-a_{nn-2}}{a_{nn-1}} & \frac{1}{a_{nn-1}} & \frac{-a_{nn}}{a_{nn-1}} \\
0 & 0 & 0 & \ldots & 0 & 0 & 1
\end{bmatrix}
$$

That is, $M$ is simply the identity matrix with the $(n-1)$'st row replaced as shown.
With a bit of staring, you should be able to convince yourself that $B = A \cdot M$ will indeed have a final row in Frobenius form.

Note that each column $l$ in $M$ has at most two non-zero elements namely $M_{ll}$ and $M_{n-1l}$
This means that the elements of $B$  are computed efficiently by considering just a couple of terms instead of the usual $n$.

$$
b_{ij} = \sum_{l=1}^{n} a_{il}m_{lj} = a_{ij}m_{jj} + a_{in-1}m_{n-1j}
$$

So

$$
b_{ij} = a_{ij} - a_{in-1} \frac{a_{nj}}{a_{nn-1}} \text{ for columns } j \ne n-1,
$$

and

$$
b_{in-1} = \frac{a_{in-1}}{a_{nn-1}} \text{ for column } n-1.
$$

Note that as promised $b_{nj} = 0 \text{ if} j \ne n-1$ and that $b_{nn-1} = 1$.

Of course, $B = A \cdot M$ is *not* similar the original matrix $A$ but $M^{-1} \cdot A \cdot M$ is.

Fortunately $M^{-1}$ is also readily computed

$$
M^{-1} =
\begin{bmatrix}
1 & 0 & 0 & \ldots & 0 & 0 & 0 \\
0 & 1 & 0 & \ldots & 0 & 0 & 0 \\
& & & \ldots \\
& & & \ldots \\
a_{n1} & a_{n2} & a_{n3} & \ldots & a_{nn-2} & a_{nn-1} & a_{nn} \\
0 & 0 & 0 & \ldots & 0 & 0 & 1
\end{bmatrix}
$$

From the form of $M^{-1}$, it is clear that the $n$'th row of $C := M^{-1} \cdot B$ is just the same as the $n$'th row of $B$, so it will be in Frobenius form.

Moreover, once again, $M^{-1}$ has at most two non-zero terms in each column.
Therefore, the matrix product can also be computed very efficiently:

$$
c_{ij} = \sum_{l=1}^{n} m_{il} b_{lj} = m_{ii} b_{ij} = b_{ij} \text{ if } i \ne n-1
$$

while

$$
c_{n-1j} = \sum_{l=1}^{n} m_{n-1l} b_{lj} = \sum_{l=1}^{n} a_{nl} b_{lj}
$$

Thus $C = M^{-1} \cdot A \cdot M$ is similar to $A$ but one step closer to companion matrix form, _and_ happily, the elements of $C$ can be efficiently computed using just $O(n^2)$ operations.
If everything goes well, we can repeat these operations for $n$ steps to arrive at the required Frobenius form shown above.
We hit a snag if $a_{nn-1} = 0$, but we will deal with that below.


### The Algorithm

. Initialize a counter $k$ to $n$ and $A$ to the input matrix.

. If $a_{kk-1} = 0$, look for an earlier element in the same row that is not zero.
That is, look for $j < k-1$ where $a_{kj} \ne 0$. \
On success, swap the rows *and* columns $j$ and $k-1$ of $A$. \
Row and column swaps like that are permutation transformations that preserve the eigen-structure. \

. If by now $a_{kk-1} \ne 0$:

.. Capture row $k$ of the matrix $A$ by setting $m = \text{row}_k(A)$. \
Note that by assumption $m_{k-1} = a_{kk-1} \ne 0$.

.. Compute the elements of $B$ for rows $i = 1, ..., k-1$ as follows:
$$
b_{ij} =
\begin{cases}
  a_{ij} -  a_{ik-1}\frac{m_j}{m_{k-1}} & \text{ if } j \ne k-1 \\
  \frac{a_{ik-1}}{m_{k-1}}              & \text{ if } j = k-1
\end{cases}
$$
You don't need any later rows of $B$.

.. Update $A$ for all columns $j = 1, \ldots, n$ as follows:
$$
\begin{aligned}
a_{ij}   &=  b_{ij} \text{ for } i = 1, \ldots, k-2, \\
a_{k-1j} &= \sum_{l=1}^{n} m_l b_{lj} = m \cdot \text{col}_j(B) \\
a_{kj}   &=
\begin{cases}
  0 & \text { for } j \ne k-1 \\
  1 & \text { for } j = k-1
\end{cases}
\end{aligned}
$$
That last step puts row $k$ of $A$ into companion matrix form --- the later rows of $A$ are already there.

.. If $k > 1$, then $k \leftarrow k-1$, and we go back to step 1. Otherwise, we are finished.

. If $a_{kk-1} = 0$ even after trying the search in step 2 then we cannot perform step 3. +
The current $A$ matrix must then have the following form:
+
$$
A =
\begin{bmatrix}
a_{11}  & a_{12} & \ldots & a_{1k-1} & a_{1k} & a_{1k+1} & \ldots & a_{1n-1} & a_{1n} \\
a_{21}  & a_{22} & \ldots & a_{2k-1} & a_{2k} & a_{2k+1} & \ldots & a_{2n-1} & a_{2n} \\
\vdots  & \vdots & \vdots & \vdots   & \vdots & \vdots   & \vdots & \vdots   & \vdots \\
0       & 0      & \ldots & 0        & a_{kk} & a_{kk+1} & \ldots & a_{kn-1} & a_{kn} \\
0       & 0      & \ldots & 0        & 1      & 0        & \ldots & 0        & 0      \\
\vdots  & \vdots & \vdots & \vdots   & \vdots & \vdots   & \vdots & \vdots   & \vdots \\
0       & 0      & \ldots & 0        & 0      & 0        & \ldots & 1        & 0
\end{bmatrix} :=
\begin{bmatrix}
A_1 & A_2 \\
0   & A_3
\end{bmatrix}
$$
+
So if $I_n$ represents the $n \times n$ identity matrix then:
+
$$
\det(\lambda I_n - A) = \det(\lambda I_{k-1} - A_1) \det(\lambda I_{n-k+1} - A_3).
$$
+
Hence the characteristic polynomial $c_A(x)$ we are after is the product of two other characteristic polynomials:
+
$$
c_A(x) = c_{A_1}(x) c_{A_3}(x)
$$
+
and as $A_3$ is already in companion form we can easily read off the coefficients for $c_{A_3}(x)$
+
$$
c_{A_3}(x) = 1 + a_{kk} x + a_{kk+1} x^2 + \ldots + a_{kn} x^{n-k+1}.
$$
+
The algorithm just stores those coefficients and recurses using $A_1$ as the smaller $(k-1) \times (k-1)$  input matrix.
+
It can then convolve the coefficients of $c_{A_1}(x)$ and $c_{A_3}(x)$ to return the coefficients for $c_{A}(x)$.

NOTE: In the case of real valued matrices it can be that $a_{kk-1}$ is non-zero but still small.
Division by very small floating point numbers should be avoided as those operations tend to be [ill-conditioned](https://en.wikipedia.org/wiki/Floating-point_arithmetic).
For that reason, step 2. might always be performed to find the $a_{kj}$ for $j < k-1$ that is largest in absolute value and then do the suggested row and column swaps to move that element into the all important $(k,k-1)$ slot.

## Danilevsky for Bit-Matrices

In the case of bit-matrices, or in more formal math-speak, matrices with elements in {f2}, the input matrix $A$ is all zeros or ones.
Moreover, the usual addition and multiplication operators are performed modulo 2 so everything remains in the limited set $\{0,1\}$. In $\mathbb{F_2}$ we can replace addition with the logical XOR operator and multiplication with the logical AND operator.

Note that in $\mathbb{F_2}$ we have $1+1 = 2 \rightarrow 0$ so the additive inverse of 1 is 1.
And of course as usual, the additive inverse of 0 is 0.
This means that in $\mathbb{F_2}$ negation is a no-op and any term like $-b$ can just be replaced with $b$.

We always have $1 * 1 = 1$ so the multiplicative inverse of $1$ is just $1$.
Also just like $\mathbb{R}$, the element $0$ has no multiplicative inverse in $\mathbb{F_2}$ either --- you still cannot divide by zero.
This means that if $a, b \in \mathbb{F_2}$ then a term like $a/b$ makes no sense if $b=0$ but otherwise $a/b = a$.

Let's reconsider that very first step we took above to move our matrix $A$ closer to Frobenius form.
That involved finding a matrix $M$ such that $B = A \cdot M$ had its final row in the required format.

Taking into account that now all the matrices are boolean and assuming that $a_{nn-1} = 1$ then the appropriate $M$ is:

$$
M =
\begin{bmatrix}
1 & 0 & 0 & \ldots & 0 & 0 & 0 \\
0 & 1 & 0 & \ldots & 0 & 0 & 0 \\
& & & \ldots \\
& & & \ldots \\
a_{n1} & a_{n2} & a_{n3} & \ldots & a_{nn-2} & a_{nn-1} & a_{nn} \\
0 & 0 & 0 & \ldots & 0 & 0 & 1
\end{bmatrix}
$$

That is, $M$ is just the identity matrix with the $(n-1)$'st row replaced with that row from $A$.

Moreover, using the fact that for any  $x \in \mathbb{F}_2$ we always have $x + x = 2x = 0$, it is  is easy to verify that $M^{-1} = M$.

So $C := M \cdot A \cdot M$ will be _similar_ to $A$ and one step closer to Frobenius form and, because $M$ is simple and sparse, those two matrix multiplications can be performed very efficiently in $O(n^2)$ operations.

The full algorithm for matrices over $\mathbb{R}$ also works for matrices over $\mathbb{F_2}$.
As before, it proceeds in a sequence of steps that move $A$ closer to companion/Frobenius matrix form at the end of each one.

### The Algorithm

1. Initialize a counter $k$ to $n$ and $A$ to the input matrix.

2. If $a_{kk-1} = 0$ look for an earlier element in the same row that is 1. That is, look for an index $j < k-1$ such that $a_{kj} = 1$. If found then swap *both* the rows and the columns $j$ and $k-1$ of $A$. These swaps are permutation transformations that preserve the eigen-structure.

3. If after step 2 we have $a_{kk-1} = 1$:

    + Capture the elements from row $k$ of the matrix $A$ by setting
$$
    m = \text{row}_k(A).
$$
      Note that by assumption $m_{k-1} = a_{kk-1} = 1$.

    + Compute the elements of $B$ for rows $i = 1, ..., k-1$ as follows
$$
b_{ij} =
\begin{cases}
  a_{ij} -  a_{ik-1}\frac{m_j}{m_{k-1}} = a_{ij} + a_{ik-1} m_j & \text{ if } j \ne k-1 \\
  \frac{a_{ik-1}}{m_{k-1}} = a_{ik-1}                           & \text{ if } j = k-1
\end{cases}
$$

    + Update $A$ for all columns $j = 1, \ldots, n$ as follows
$$
\begin{aligned}
a_{ij}   &=  b_{ij} \text{ for } i = 1, \ldots, k-2, \\
a_{k-1j} &= \sum_{l=1}^{n} m_l b_{lj} = m \cdot \text{col}_j(B) \\
a_{kj}   &=
\begin{cases}
  0 & \text { for } j \ne k-1 \\
  1 & \text { for } j = k-1
\end{cases}
\end{aligned}
$$
That last step puts row $k$ of $A$ into Frobenius form --- later rows are already there.

    + If $k > 1$ then $k \gets k-1$ and we go back to step 1, otherwise, we are done.

4. If after step 2 we have $a_{kk-1} = 0$ then we cannot perform step 3. \
In this case, the current $A$ matrix must have the following form:
$$
A =
\begin{bmatrix}
A_1 & A_2 \\
0   & A_3
\end{bmatrix}
$$
hence the characteristic polynomial $c_A(x)$ is the product of two others: \
$$
c_A(x) = c_{A_1}(x) c_{A_3}(x).
$$
As $A_3$ is already in Frobenius form we can easily read off the coefficients for $c_{A_3}(x)$: \
$$
c_{A_3}(x) = 1+ a_{kk} x + a_{kk+1} x^2 + \ldots + a_{kn} x^{n-k+1}.
$$
Store those coefficients and recurse using $A_1$ as the $(k-1) \times (k-1)$ input matrix.
Convolve the coefficients of $c_{A_1}(x)$ and $c_{A_3}(x)$ to get the coefficients for $c_{A}(x)$.

NOTE: In {f2} any matrix element can only be $0$ or $1$.
Therefore, all things being equal, you'd expect to have to perform the recursive fourth step half the time.
